Fix runtime bug -- lean_dec on uninit array elems

bindings/leancolls_array.c
@@ -2,7 +2,23 @@
 #include <string.h>
 #include <stdlib.h>
 
-// Declare array class
+/*
+ArrayUninit C implementation
+
+Representation specified by three things:
+  - uint64 n: length 
+  - uint64 m: m <= n, "filled" length
+  - lean_object*[n] backing:
+    for 0 <= i < m, backing[i] is initialized with a valid lean_object*
+    for m <= i < n, backing[i] is uninitialized
+
+TODO: Eventually we may be able to ensure that the finalizer is
+only called if all elements are uninitialized. Then we could
+generalize to avoid the m parameter entirely, and let the
+initialization status be a noncomputable property of the use code.
+*/
+
+// Declare external class
 
 static lean_external_class* leancolls_array_external_class = NULL;
 
@@ -25,13 +41,37 @@ lean_obj_res leancolls_array_initialize()
 
 // Getting into/out of lean_obj*
 
-lean_obj_res leancolls_array_box(lean_object** arr)
-{
+lean_obj_res leancolls_array_box(lean_object** arr) {
     return lean_alloc_external(leancolls_array_external_class, arr);
 }
 
 lean_object** leancolls_array_unbox(lean_obj_arg o) {
+    assert (lean_is_external(o));
     return (lean_object**)(lean_get_external_data(o));
+}
+
+static inline size_t leancolls_array_unbox_size(b_lean_obj_arg n) {
+    // On both 64bit and 32bit systems, if n is not scalar this would OOM
+    if (!lean_is_scalar(n)) {
+        lean_internal_panic_out_of_memory();
+    }
+
+    size_t len = (size_t)(lean_unbox(n));
+    if (len != sizeof(lean_object*) * len / sizeof(lean_object*)) {
+        lean_internal_panic_out_of_memory();
+    }
+
+    return len;
+}
+
+
+// Exclusivity checking
+
+uint8_t leancolls_array_isexclusive(b_lean_obj_arg n, b_lean_obj_arg m, b_lean_obj_arg a) {
+    if (lean_is_exclusive(a))
+        return 1;
+    else
+        return 0;
 }
 
 static inline void leancolls_array_ensure_exclusive(lean_obj_arg a) {
@@ -49,26 +89,12 @@ static inline void leancolls_array_ensure_exclusive(lean_obj_arg a) {
     }
 }
 
-static inline size_t leancolls_unbox_array_size(b_lean_obj_arg n) {
-    // On both 64bit and 32bit systems, if n is not scalar this would OOM
-    if (!lean_is_scalar(n)) {
-        lean_internal_panic_out_of_memory();
-    }
-
-    size_t len = (size_t)(lean_unbox(n));
-    if (len != sizeof(lean_object*) * len / sizeof(lean_object*)) {
-        lean_internal_panic_out_of_memory();
-    }
-
-    return len;
-}
-
 
 // Implement basic external functions
 
-lean_obj_res leancolls_array_new_uninit(b_lean_obj_arg n) {
+lean_obj_res leancolls_array_new(b_lean_obj_arg n) {
 
-    size_t len = leancolls_unbox_array_size(n);
+    size_t len = leancolls_array_unbox_size(n);
 
     lean_object** backing = malloc(sizeof(lean_object*) * len);
     // Check if malloc failed
@@ -81,52 +107,94 @@ lean_obj_res leancolls_array_new_uninit(b_lean_obj_arg n) {
     return leancolls_array_box(backing);
 }
 
-
-lean_obj_res leancolls_array_new(b_lean_obj_arg x, b_lean_obj_arg n) {
-
-    size_t len = leancolls_unbox_array_size(n);
-
-    lean_object** backing = malloc(sizeof(lean_object*) * len);
-    // Check if malloc failed
-    if (backing == NULL) {
-        lean_panic_fn(NULL, lean_mk_string(
-            "LeanColls.Array: New allocation failed! (Out of memory?)"
-        ));
-    }
-
-    // Initialize
-    if (lean_is_scalar(x)) {
-        for (size_t i = 0; i < len; i++) {
-            backing[i] = x;
-        }
-    } else {
-        for (size_t i = 0; i < len; i++) {
-            lean_inc(x);
-            backing[i] = x;
-        }
-    }
-
-    return leancolls_array_box(backing);
-}
-
-lean_obj_res leancolls_array_get(b_lean_obj_arg len, b_lean_obj_arg arr, b_lean_obj_arg i) {
-    // `len` is scalar; non-scalar `len` will OOM (see `leancolls_unbox_array_size`)
+// Assuming `arr[i]` is initialized, retrieve it
+lean_obj_res leancolls_array_get(
+    b_lean_obj_arg len, b_lean_obj_arg filled,
+    b_lean_obj_arg arr, b_lean_obj_arg i
+) {
+    // `len` is scalar; non-scalar `len` will OOM (see `leancolls_array_new`)
     assert(lean_is_scalar(len));
-    // `(i : Fin len)` so `i` should be a scalar less than `len`
+    // `filled <= len` (an invariant that should be maintained)
+    assert(lean_is_scalar(filled));
+    assert(lean_unbox(filled) <= lean_unbox(len));
+    // `i < filled`
     assert(lean_is_scalar(i));
-    assert(lean_unbox(i) < lean_unbox(len)); // (Could compare boxed values directly but...)
+    assert(lean_unbox(i) < lean_unbox(filled));
+    // `arr` is an external obj
+    assert(lean_is_external(arr));
 
-    lean_object* a = (leancolls_array_unbox(arr))[lean_unbox(i)];
+    lean_object** backing = leancolls_array_unbox(arr);
+
+    size_t i_ = lean_unbox(i);
+
+    lean_object* a = backing[i_];
     lean_inc(a);
     return a;
 }
 
-lean_obj_res leancolls_array_set(b_lean_obj_arg len, lean_obj_arg arr, b_lean_obj_arg i, lean_obj_arg a) {
-    // `len` is scalar; non-scalar `len` will OOM (see `new`)
+lean_obj_res leancolls_array_push(
+    b_lean_obj_arg len, b_lean_obj_arg filled,
+    lean_obj_arg arr, lean_obj_arg a
+) {
+    // `len` is scalar; non-scalar `len` will OOM (see `leancolls_array_new`)
     assert(lean_is_scalar(len));
-    // `(i : Fin len)` so `i` should be a scalar less than `len`
+    // `filled < len`
+    assert(lean_is_scalar(filled));
+    assert(lean_unbox(filled) < lean_unbox(len));
+    // `arr` is an external obj
+    assert(lean_is_external(arr));
+
+    leancolls_array_ensure_exclusive(arr);
+
+    lean_object** backing = leancolls_array_unbox(arr);
+
+    size_t i_ = lean_unbox(filled);
+
+    // Insert new value; old value is uninitialized.
+    backing[i_] = a;
+
+    return arr;
+}
+
+lean_obj_res leancolls_array_pop(
+    b_lean_obj_arg len, b_lean_obj_arg filled,
+    lean_obj_arg arr
+) {
+    // `len` is scalar; non-scalar `len` will OOM (see `leancolls_array_new`)
+    assert(lean_is_scalar(len));
+    // `0 < filled <= len`
+    assert(lean_is_scalar(filled));
+    assert(0 < lean_unbox(filled));
+    assert(lean_unbox(filled) <= lean_unbox(len));
+    // `arr` is an external obj
+    assert(lean_is_external(arr));
+
+    leancolls_array_ensure_exclusive(arr);
+
+    lean_object** backing = leancolls_array_unbox(arr);
+
+    size_t i_ = lean_unbox(filled);
+
+    // Throw out old initialized value
+    lean_dec(backing[i_ - 1]);
+
+    return arr;
+}
+
+lean_obj_res leancolls_array_set(
+    b_lean_obj_arg len, b_lean_obj_arg filled,
+    lean_obj_arg arr, b_lean_obj_arg i, lean_obj_arg a
+) {
+    // `len` is scalar; non-scalar `len` will OOM (see `leancolls_array_new`)
+    assert(lean_is_scalar(len));
+    // `filled <= len`
+    assert(lean_is_scalar(filled));
+    assert(lean_unbox(filled) <= lean_unbox(len));
+    // `i < filled`
     assert(lean_is_scalar(i));
-    assert(lean_unbox(i) < lean_unbox(len)); // (Could compare boxed values directly but...)
+    assert(lean_unbox(i) < lean_unbox(filled));
+    // `arr` is an external obj
+    assert(lean_is_external(arr));
 
     leancolls_array_ensure_exclusive(arr);
 
@@ -144,10 +212,21 @@ lean_obj_res leancolls_array_set(b_lean_obj_arg len, lean_obj_arg arr, b_lean_ob
     return arr;
 }
 
-lean_object* leancolls_array_resize(b_lean_obj_arg n, lean_obj_arg arr,
-                                    b_lean_obj_arg x, b_lean_obj_arg m) {
-    size_t old_len = leancolls_unbox_array_size(n);
-    size_t new_len = leancolls_unbox_array_size(m);
+lean_object* leancolls_array_resize(
+    b_lean_obj_arg len, b_lean_obj_arg filled,
+    lean_obj_arg arr, b_lean_obj_arg len_
+) {
+    // `len` is scalar; non-scalar `len` will OOM (see `leancolls_array_unbox_size`)
+    assert(lean_is_scalar(len));
+    // filled <= len
+    assert(lean_is_scalar(filled));
+    assert(lean_unbox(filled) <= lean_unbox(len));
+
+    size_t old_len = lean_unbox(len);
+    size_t new_len = leancolls_array_unbox_size(len_);
+
+    // filled <= len_ (so that no initialized elements are dropped)
+    assert(lean_unbox(filled) <= new_len);
 
     leancolls_array_ensure_exclusive(arr);
 
@@ -160,18 +239,6 @@ lean_object* leancolls_array_resize(b_lean_obj_arg n, lean_obj_arg arr,
         lean_panic_fn(NULL, lean_mk_string(
             "LeanColls.Array: Reallocation failed! (Out of memory?)"
         ));
-    }
-
-    // Initialize
-    if (lean_is_scalar(x)) {
-        for (size_t i = old_len; i < new_len; i++) {
-            new_backing[i] = x;
-        }
-    } else {
-        for (size_t i = old_len; i < new_len; i++) {
-            lean_inc(x);
-            new_backing[i] = x;
-        }
     }
 
     return leancolls_array_box(new_backing);
