LeanColls/Array/Basic.lean
@@ -10,77 +10,126 @@ import LeanColls.IndexedOps
 import LeanColls.Uninit
 import LeanColls.AuxLemmas
 import LeanColls.View
+import LeanColls.Array.ArrayUninit
 
 namespace LeanColls
 
-@[extern "leancolls_array_initialize"] private opaque arrayInit : IO Unit
+/-! # Fixed-length arrays
 
-builtin_initialize arrayInit
-
+Represented as an `ArrayUninit`.
+-/
 structure Array (α : Type u) (n : Nat) : Type u where
-  data : (i : Fin n) → α
+  data : ArrayUninit α n n (Nat.le_refl _)
 
 namespace Array
 
-instance [Inhabited α] : Inhabited (Array α n) where
-  default := ⟨fun _ => default⟩
+/-!
+### Array.new
 
--- External functions
+Build an array of length `n` where all elements are instantiated to `x`.
+-/
+def new (x : α) (n : Nat) : Array α n :=
+  have res := Range.foldl'' ⟨n⟩
+    (motive := fun i => Σ' h, Σ' (A : ArrayUninit α n i h),
+      ∀ j hm, A.get j (Nat.lt_of_lt_of_le hm h) hm = x)
+    (fun _ h_i ⟨_, A, h⟩ =>
+      ⟨h_i, A.push x h_i, by
+        intro j hm
+        simp
+        split; rfl; apply h⟩
+    ) ⟨Nat.zero_le _, ArrayUninit.new n, by intro _ hj; contradiction⟩
+  ⟨res.2.1⟩
 
-@[extern "leancolls_array_new_uninit"]
-def newUninit (n : Nat) : Array (Uninit α) n
-  := ⟨λ _ => Uninit.uninit⟩
+/-!
+### Array.init
 
-@[extern "leancolls_array_new"]
-def new (x : @&α) (n : @& Nat) : Array α n
-  := ⟨λ _ => x⟩
+Build an array of length `n` where element `i` is instantiated to `f i`.
+-/
+def init {α : Type u} {n : Nat} (f : Fin n → α) : Array α n :=
+  have res := Range.foldl'' ⟨n⟩
+    (motive := fun i => Σ' h, Σ' (A : ArrayUninit α n i h),
+      ∀ j hm, A.get j (Nat.lt_of_lt_of_le hm h) hm =
+              f ⟨j,(Nat.lt_of_lt_of_le hm h)⟩)
+    (fun i h_i ⟨_, A, h⟩ =>
+      ⟨h_i, A.push (f ⟨i,h_i⟩) h_i, by
+        intro j hj
+        simp
+        have := Nat.lt_or_eq_of_le <| Nat.le_of_succ_le_succ hj
+        cases this
+        case inr hj => simp [hj]
+        case inl hj =>
+          simp [Nat.ne_of_lt hj]
+          apply h⟩
+    ) ⟨Nat.zero_le _, ArrayUninit.new n, by intro _ hj; contradiction⟩
+  ⟨res.2.1⟩
 
-@[extern "leancolls_array_get"]
-def get {α} {n : @& Nat}
-        (A : @& Array α n) (i : @& Fin n) : α
-  := A.data i
+/-!
+### Array.get
 
-@[extern "leancolls_array_set"]
-def set {α} {n : @& Nat}
-        (A : Array α n) (i : @& Fin n) (x : α)
-  : Array α n
-  := ⟨λ a => if a = i then x  else A.data a⟩
+Gets an element at the specified index. An array is uniquely characterized
+by its `get` (see `Array.ext`).
+-/
+@[inline]
+def get (A : @& Array α n) (i : @& Fin n) : α
+  := A.data.get i.val i.isLt i.isLt
 
-@[extern "leancolls_array_resize"]
-def resize {α} {n : @& Nat} (A : Array α n)
-          (x : @&α) (m : @& Nat)
-  : Array α m
-  := ⟨λ i => if h:i < n
-    then A.data ⟨i,h⟩
-    else x⟩
+/-!
+### Array.set
 
-unsafe def allInitUnsafe (A : Array (Uninit α) n)
-  (_ : ∀ i, (A.get i).isInit) : Array α n
-  := unsafeCast A
-@[implementedBy allInitUnsafe]
-def allInit (A : Array (Uninit α) n)
-  (h : ∀ i, (A.get i).isInit) : Array α n
-  := ⟨λ i => Uninit.getValue (A.get i) (h i)⟩
+Sets the element at index `i` to `x`, throwing out the old value.
+-/
+@[inline]
+def set {n : @& Nat} (A : Array α n) (i : @& Fin n) (x : α) : Array α n
+  := ⟨A.data.set i i.isLt x⟩
 
--- Axioms
+/-!
+## Extensionality & simp lemmas
+-/
 
-/- This axiom holds, because instantiating an array of at least `USize.size`
-  will cause the program to panic -/
-axiom size_lt_usize {α n} : Array α n → n < USize.size
+@[simp]
+theorem ext {α n} {A B : Array α n} : A = B ↔ A.get = B.get
+  := by
+  constructor
+  intro h; rw [h]
+  intro h; cases A; cases B
+  simp [get] at h ⊢
+  funext i h_i _
+  exact congrFun h ⟨i,h_i⟩
 
--- Preliminary theorems
+@[simp]
+theorem get_new {x : α} {n} {i : Fin n}
+  : get (new x n) i = x
+  := by
+  simp [get, new]
+  generalize Range.foldl'' _ _ _ _ = res
+  match res with
+  | ⟨_, _, h⟩ =>
+  simp
+  apply h
+
+@[simp]
+theorem get_init {f : Fin n → α} {i}
+  : get (init f) i = f i
+  := by
+  simp [get, init]
+  generalize Range.foldl'' _ _ _ _ = res
+  match res with
+  | ⟨_, _, h⟩ =>
+  simp
+  apply h
+
 theorem get_of_set_eq (f : Array α n) (i : Fin n) (x : α) {i' : Fin n} (h_i : i = i')
   : (f.set i x).get i' = x
-  := by unfold get; unfold set; simp [h_i, Function.update, cast]
+  := by
+  simp [get, set, ArrayUninit.get_set, h_i]
 
 theorem get_of_set_ne (f : Array α n) (i : Fin n) (x : α) (j : Fin n) (h : i ≠ j)
   : (f.set i x).get j = f.get j
   := by
-    unfold get; unfold set
-    simp [Function.update]
-    split
-    exact False.elim $ h (by apply Eq.symm; assumption)
-    rfl
+  simp [get, set]
+  cases i; cases j
+  simp at h ⊢
+  simp [h]
 
 @[simp]
 theorem get_of_set (f : Array α n) (i : Fin n) (x : α) {i' : Fin n}
@@ -90,104 +139,17 @@ theorem get_of_set (f : Array α n) (i : Fin n) (x : α) {i' : Fin n}
   apply get_of_set_eq; assumption
   apply get_of_set_ne; assumption
 
-/-!
-### Array.init
-
-Utility function necessary to provide a runtime implementation
-for `Array.mk`.
--/
-@[inline]
-def init {α : Type u} {n : Nat} (f : Fin n → α) : Array α n
-  :=
-  Range.foldl' ⟨n⟩ (λ A' i h => A'.set ⟨i,h⟩ (.init $ f ⟨i,h⟩)) (newUninit n)
-  |>.allInit (by
-    intro i
-    cases i; case mk i hi =>
-    simp [newUninit]
-    suffices ∀ n' (hn : ∀ {i}, i < n' → i < n) (_ : i < n'),
-      Uninit.isInit (
-        get
-          (Range.foldl'
-            ⟨n'⟩
-            (fun A i h => A.set ⟨i, hn h⟩ (.init $ f ⟨i, hn h⟩))
-            (⟨λ _ => Uninit.uninit⟩ : Array (Uninit α) n))
-          ⟨i, hi⟩)
-      from this n (by simp) hi
-    intro n' hn hi'
-    induction n' with
-    | zero =>
-      contradiction
-    | succ n' ih =>
-      simp at hi
-      simp [Range.foldl']
-      match Nat.eq_or_lt_of_le hi' with
-      | .inl h =>
-        cases h
-        simp
-      | .inr h =>
-        have : i < n' := Nat.le_of_succ_le_succ h
-        simp [(Nat.ne_of_lt this).symm]
-        apply ih
-        exact this
-    )
-
-/-!
-Implement the auto-generated `mk` and `data` functions with
-actually-correct implementations above. This seals up all
-routes to interact with the `Array`, ensuring safety.
--/
-attribute [implementedBy init] Array.mk
-def dataImpl {α : Type u} {n : Nat}
-        (A : Array α n) (i : Fin n) : α
-  := A.get i
-attribute [implementedBy dataImpl] Array.data
-def recImpl.{u_1,u}
-  : {α : Type u} → {n : Nat} → {motive : Array α n → Sort u_1} →
-    ((data : Fin n → α) → motive ⟨data⟩) →
-    (t : Array α n) → motive t
-  := λ f A => f (data A)
-attribute [implementedBy recImpl] Array.rec
-
-theorem init_eq_mk {f : Fin n → α}
-  : init f = Array.mk f
-  := by
-    simp [init, forIn, Foldable.fold, Id.run, allInit]
-    apply funext; intro i
-    cases i; case mk i hi =>
-    suffices ∀ n' (hn : ∀ {i}, i < n' → i < n) (hi' : i < n'),
-      Uninit.getValue?
-        (get (Range.foldl' ⟨n'⟩ (fun A' i h =>
-                set A' ⟨i,hn h⟩ (Uninit.init (f ⟨i,hn h⟩))
-              ) (newUninit n)
-          ) ⟨i, hn hi'⟩)
-        = some (f ⟨i, hi⟩)
-      by
-      apply Uninit.getValue_of_getValue?_some
-      exact this n (by simp) hi
-    intro n' hn hi'
-    induction n' with
-    | zero =>
-      contradiction
-    | succ n' ih =>
-      simp [Range.foldl']
-      match Nat.eq_or_lt_of_le (Nat.le_of_succ_le_succ hi') with
-      | .inl hi' =>
-        cases hi'
-        simp [Uninit.getValue?_init]
-      | .inr hi' =>
-        simp [(Nat.ne_of_lt hi').symm]
-        apply ih
-        assumption
-
 def empty : Array α 0 := init (Fin.elim0)
 
 def copy {n : Nat} (A : Array α n) : Array α n
   := init A.get
 
+@[simp]
 theorem copy_def (A : Array α n) : A.copy = A
   := by
-  simp [copy, init_eq_mk]
-  rfl
+  simp [copy]
+  funext i
+  simp
 
 instance : Indexed (Array α n) α where
   size _ := n
@@ -195,10 +157,68 @@ instance : Indexed (Array α n) α where
 
 instance : IndexedOps (Array α n) α := default
 
+instance [N : Nonempty α] : Nonempty (Array α n) :=
+  Nonempty.elim N (fun a => ⟨new a n⟩)
+
+instance [Inhabited α] : Inhabited (Array α n) where
+  default := new default n
+
 def toList (A : Array α n) : List α := FoldableOps.toList A
 
+def ofList (L : List α) : Array α L.length :=
+  have res :=
+    (Range.mk L.length).foldl''
+      (motive := fun i =>
+        Σ' h, Σ' (acc : ArrayUninit α L.length i h) (rest : List α),
+        rest = L.drop i ∧ ∀ j h_j,
+        acc.get j (Nat.lt_of_lt_of_le h_j h) h_j =
+          L.get ⟨j, Nat.lt_of_lt_of_le h_j h⟩)
+      (fun i h ⟨_, acc, rest, h_rest, h_acc⟩ =>
+        match rest with
+        | [] => False.elim <| by
+          have := List.length_drop i L
+          rw [←h_rest] at this
+          simp at this
+          apply Nat.ne_of_lt h
+          apply Nat.le_antisymm
+          exact Nat.le_of_lt h
+          exact Nat.sub_eq_zero_iff_le.mp this.symm
+        | x::rest =>
+          ⟨h, acc.push x h
+          , rest
+          , by
+            have := h_rest.symm ▸ List.get_drop_eq_drop L i h
+            have h_x : x = L[i]' h := by
+              simp at this; exact this.1.symm
+            have h_rest : rest = L.drop i.succ := by
+              simp at this; exact this.2.symm
+            constructor
+            exact h_rest
+            intro j h_j
+            simp
+            split
+            subst_vars
+            simp [getElem', getElem]
+            apply h_acc
+            ⟩
+      )
+      ⟨Nat.zero_le _, ArrayUninit.new _, L, by simp,
+        by intro j hj; contradiction⟩
+  ⟨res.2.1⟩
+
+@[simp]
+theorem get_ofList (L : List α) (i)
+  : get (ofList L) i = L.get i
+  := by
+  simp [get, ofList]
+  generalize Range.foldl'' _ _ _ _ = res
+  match res with
+  | ⟨h, acc, rest, h_rest, h_acc⟩ =>
+  simp
+  apply h_acc
+
 instance [Repr α] : Repr (Array α n) where
-  reprPrec A := reprPrec (α := List α) A.toList
+  reprPrec A prec := "Array.ofList " ++ reprPrec (α := List α) A.toList prec
 
 @[simp]
 theorem canonicalToList_eq_toList (A : Array α n)
@@ -212,6 +232,9 @@ theorem canonicalToList_eq_toList (A : Array α n)
 theorem size_set (A : Array α n) (i : Fin n) (x : α)
   : Size.size (A.set i x) = Size.size A
   := by simp [Size.size]
+
+@[simp]
+def length (_ : Array α n) := n
 
 @[simp]
 theorem length_toList (A : Array α n)
