LeanColls/Array/ArrayBuffer.lean
@@ -4,92 +4,70 @@ namespace LeanColls
 
 structure ArrayBuffer (α) where
   cap : Nat
-  h_cap : 1 ≤ cap
-  size : Fin cap.succ
-  backing : Array (Uninit α) cap
-  h_filled : ∀ i, (h : i < size.val) →
-    backing.get ⟨i, Nat.lt_of_lt_le h <| Nat.le_of_succ_le_succ size.isLt⟩
-    |>.isInit
+  h_cap : cap > 0
+  size : Nat
+  h_size : size ≤ cap
+  backing : ArrayUninit α cap size h_size
 
 namespace ArrayBuffer
 
 def empty (_ : Unit) (initCap : Nat := 16) (h_cap : 1 ≤ initCap := by decide) : ArrayBuffer α := ⟨
   initCap,
   h_cap,
-  ⟨0, Nat.le_step h_cap⟩,
-  Array.new (Uninit.uninit) initCap,
-  by intro i h; simp [Fin.val] at h; contradiction
+  0,
+  Nat.zero_le _,
+  ArrayUninit.new initCap
   ⟩
 
-@[inline] def full (A : ArrayBuffer α) : Bool := A.size.val = A.cap
+@[inline] def full (A : ArrayBuffer α) : Bool := A.size = A.cap
 
 def grow : ArrayBuffer α → ArrayBuffer α :=
-λ ⟨cap, h_cap, size, backing, h_backing⟩ =>
+λ ⟨cap, h_cap, size, h_size, backing⟩ =>
   let newCap := 2 * cap
   have : cap < newCap := by
     have := Nat.mul_lt_mul_of_pos_right (Nat.lt_succ_self 1) h_cap
     simp at this ⊢
     assumption
   ⟨newCap, Nat.le_trans h_cap <| Nat.le_of_lt this,
-    ⟨size, Nat.lt_trans size.isLt $ Nat.succ_lt_succ this⟩,
-    backing.resize (Uninit.uninit) newCap,
-    by
-      intro i h
-      simp at h
-      have : i < cap := Nat.lt_of_lt_le h (Nat.le_of_succ_le_succ size.isLt)
-      simp [Array.get, Array.resize, this]
-      apply h_backing
-      assumption
-      ⟩
+    size,
+    Nat.le_trans h_size <| Nat.le_of_lt this,
+    backing.resize newCap (Nat.le_trans h_size <| Nat.le_of_lt this)⟩
 
 theorem grow_notfull (A : ArrayBuffer α)
   : ¬A.grow.full
   := by
     simp [full,grow]
     apply (decide_eq_false_iff_not _).mpr
-    suffices A.size.val < 2 * A.cap from
+    suffices A.size < 2 * A.cap from
       Nat.ne_of_lt this
     have := Nat.mul_lt_mul_of_pos_right (Nat.lt_succ_self 1) A.h_cap
     simp at this ⊢
-    apply Nat.lt_of_le_of_lt (Nat.le_of_succ_le_succ A.size.isLt)
+    apply Nat.lt_of_le_of_lt A.h_size
     assumption
 
 @[inline] def push_notfull (A : ArrayBuffer α) (h : ¬A.full) (a : α) : ArrayBuffer α
   :=
     match A with
-    | ⟨cap, h_cap, size, backing, h_backing⟩ =>
-    have h_size :=
-      Nat.le_of_lt_succ $
-      Nat.lt_of_le_of_ne size.isLt (by
-      simp [full] at h; intro h'; apply h; injection h'; assumption)
-    ⟨ cap, h_cap, ⟨size.val + 1, Nat.succ_le_succ h_size⟩,
-      backing.set ⟨size,h_size⟩ (Uninit.init a),
-      by
-        intro i h_i
-        cases size; case mk size _ =>
-        by_cases h : i = size
-        cases h
-        rw [backing.get_of_set_eq]
-        exact Uninit.isInit_init
-        simp [Fin.eq_of_val_eq]
-        rw [backing.get_of_set_ne _ _ _ (by simp; exact h ∘ Eq.symm)]
-        have h_i : i < size := Nat.lt_of_le_of_ne (Nat.le_of_succ_le_succ h_i) h
-        exact h_backing i h_i⟩
+    | ⟨cap, h_cap, size, h_size, backing⟩ =>
+    have h_size : size < cap :=
+      Nat.lt_of_le_of_ne h_size <| by simp [full] at h; exact h
+    ⟨ cap, h_cap,
+      size + 1, h_size,
+      backing.push a h_size⟩
 
 def push (A : ArrayBuffer α) (a : α) : ArrayBuffer α :=
-  if h:A.size.val = A.cap then
+  if h:A.size = A.cap then
     A.grow.push_notfull (A.grow_notfull) a
   else
     A.push_notfull (by simp [full,h]) a
 
-
 def toArray (A : ArrayBuffer α) : Array α A.size :=
-  A.backing.resize (unreachable!) A.size
-  |>.allInit <| by
-    intro ⟨i,h_i⟩
-    have : i < A.cap := Nat.lt_of_lt_le h_i <| Nat.le_of_succ_le_succ A.size.isLt
-    simp [Array.resize, Array.get, this]
-    exact A.h_filled _ h_i
+  match A with
+  | ⟨_, _, size, h_size, backing⟩ =>
+  if backing.isExclusive
+  then ⟨backing.resize size (Nat.le_refl _)⟩
+  else Array.init (n := size) (fun ⟨i,h⟩ =>
+    backing.get i (Nat.lt_of_lt_of_le h h_size) h)
 
 end ArrayBuffer
 
