LeanColls/Array/ArrayUninit.lean
@@ -1,0 +1,81 @@
+/-
+Copyright (c) 2022 James Gallicchio.
+
+Authors: James Gallicchio
+-/
+
+import LeanColls.Classes
+import LeanColls.Range
+import LeanColls.IndexedOps
+import LeanColls.Uninit
+import LeanColls.AuxLemmas
+import LeanColls.View
+
+namespace LeanColls
+
+@[extern "leancolls_array_initialize"] private opaque arrayInit : IO Unit
+
+builtin_initialize arrayInit
+
+opaque ArrayUninit.Pointed (α : Type u) (n m : Nat) (h : m ≤ n): NonemptyType.{u}
+
+def ArrayUninit (α) (n m : Nat) (h : m ≤ n) := (ArrayUninit.Pointed α n m h).type
+
+namespace ArrayUninit
+
+instance : Nonempty (ArrayUninit α n m h) := (ArrayUninit.Pointed α n m h).property
+
+axiom partiallyInit_inhabited {α n m h} (A : ArrayUninit α n (.succ m) h) : Inhabited α
+
+@[extern "leancolls_array_new"]
+opaque new (n : @& Nat) : ArrayUninit α n 0 (Nat.zero_le _)
+
+@[extern "leancolls_array_get"]
+opaque get {n m : @& Nat} {h} (A : @& ArrayUninit α n m h) (i : @& Nat) (h_in : i < n) (h_im : i < m) : α
+  := match m with
+  | 0 => by contradiction
+  | m+1 => (partiallyInit_inhabited A).default
+
+@[extern "leancolls_array_push"]
+opaque push {n m : @& Nat} {h} (A : ArrayUninit α n m h) (x : α) (h' : m < n) : ArrayUninit α n m.succ h'
+
+@[extern "leancolls_array_pop"]
+opaque pop {n m : @& Nat} {h} (A : ArrayUninit α n m.succ h) : ArrayUninit α n m (Nat.le_of_succ_le h)
+
+@[extern "leancolls_array_set"]
+opaque set {n m : @& Nat} {h} (A : ArrayUninit α n m h) (i : @& Nat) (h_i : i < n) (x : α) : ArrayUninit α n m h
+
+@[extern "leancolls_array_resize"]
+opaque resize {n m : @& Nat} {h} (A : ArrayUninit α n m h) (n' : @& Nat) (h' : m <= n') : ArrayUninit α n' m h'
+
+@[extern "leancolls_array_isexclusive"]
+opaque isExclusive {n m : @& Nat} {h} (A : @& ArrayUninit α n m h) : Bool
+
+@[simp]
+axiom get_push {α n m h} {A : ArrayUninit α n m h} {x h' i hn hm}
+  : get (push A x h') i hn hm =
+    if h_i : i = m then x
+    else get A i hn (Nat.lt_of_le_of_ne (Nat.le_of_succ_le_succ hm) h_i)
+
+@[simp]
+axiom get_pop {α n m h} {A : ArrayUninit α n (.succ m) h} {i hn hm}
+  : get (pop A) i hn hm = get A i hn (Nat.le_step hm)
+
+@[simp]
+axiom get_set {α n m h} {A : ArrayUninit α n m h} {i hi x j hn hm}
+  : get (set A i hi x) j hn hm =
+    if i = j then x
+    else get A j hn hm
+
+@[simp]
+axiom get_resize {α n m h} {A : ArrayUninit α n m h} {n' h' i hn hm}
+  : get (resize A n' h') i hn hm = get A i (Nat.lt_of_lt_of_le hm h) hm
+
+axiom ext {α n m h} {A B : ArrayUninit α n m h} : A.get = B.get → A = B
+
+@[simp]
+theorem ext_iff {α n m h} {A B : ArrayUninit α n m h}
+  : A = B ↔ A.get = B.get := by
+  constructor
+  intro eq; rw [eq]
+  exact ext
